WIP in inline proof

theories/L6_PCPS/inline_correct.v
@@ -49,11 +49,11 @@ Section Inline_Eq.
        | (true, Some (t, xs, e), S d') =>
          let sig' := set_list (combine xs ys') sig  in            
          e' <- beta_contract _ IH d' e sig' fm s' ;;
-         match inline_letapp e' x with
-         | Some (C, x') =>
+         match inline_letapp e' x, Nat.eqb (List.length xs) (List.length ys) with
+         | Some (C, x'), true =>
            ec' <- beta_contract _ IH d' ec (M.set x x' sig) fm s' ;;
            ret (C |[ ec' ]|)
-         | None =>
+         | _, _ =>
            x' <- get_name x "" ;;
            ec' <- beta_contract _ IH d ec (M.set x x' sig) fm s' ;;
            ret (Eletapp x' f' t ys' ec')
@@ -87,9 +87,11 @@ Section Inline_Eq.
       let ys' := apply_r_list sig ys in
       let (s', inl) := update_App _ IH f' t ys' s in
       (match (inl, M.get f fm, d) with
-       | (true, Some (t, xs, e), S d') =>
-         let sig' := set_list (combine xs ys') sig  in
-         beta_contract _ IH d' e sig' fm  s'
+       | (true, Some (ft, xs, e), S d') =>
+         if Nat.eqb (List.length xs) (List.length ys) then
+           let sig' := set_list (combine xs ys') sig  in
+           beta_contract _ IH d' e sig' fm  s'
+         else ret (Eapp f' t ys')
        | _ => ret (Eapp f' t ys')
        end)
     | Eprim x t ys e =>
@@ -180,12 +182,12 @@ Section Inline_correct.
 
   Definition occurs_free_in_val (v : val) : Ensemble var :=
     match v with
-    | Vfun rho B f => occurs_free_fundefs B
+    | Vfun rho B f => occurs_free_fundefs B :|: name_in_fundefs B
     | _ => Empty_set _
     end.
     
   Definition occurs_free_in_env (rho : env) : Ensemble var :=
-    fun v => exists x r B f, rho!x = Some (Vfun r B f) /\ v \in occurs_free_fundefs B.
+    fun v => exists x r B f, rho!x = Some (Vfun r B f) /\ v \in occurs_free_fundefs B :|: name_in_fundefs B.
 
   Definition fun_bindings_val (v : val) :=
     match v with
@@ -248,80 +250,100 @@ Section Inline_correct.
     - simpl in HIn. now right.
   Qed.
 
-  Fixpoint fun_map_inv' (k : nat) (S : Ensemble var) (fm : fun_map) (rho : env) : Prop :=
+  Fixpoint fun_map_inv' (k : nat) (S : Ensemble var) (fm : fun_map) (rho1 rho2 : env) (i : nat) (sig : subst) : Prop :=
     forall f ft xs e rhoc B f',
       f \in S ->
       fm ! f = Some (ft, xs, e) ->
-      rho ! f = Some (Vfun rhoc B f') ->
+      rho1 ! f = Some (Vfun rhoc B f') ->
       find_def f B = Some (ft, xs, e) /\ f = f' /\
-      eq_env_P (occurs_free_fundefs B) rho rhoc /\      
+      preord_env_P_inj cenv PG (name_in_fundefs B :|: occurs_free_fundefs B) i (apply_r sig) (def_funs B B rhoc rhoc) rho2 /\
+      sub_map (def_funs B B rhoc rhoc) rho1 /\
+      Disjoint _ (bound_var e) (name_in_fundefs B :|: FromList xs :|: occurs_free_in_env rho1 :|: Dom_map rhoc) /\
+      Disjoint _ (FromList xs) (name_in_fundefs B :|: occurs_free_in_env rho1 :|: Dom_map rhoc :|: Dom_map fm) /\
       match k with
       | 0%nat => True
-      | S k => fun_map_inv' k (occurs_free_fundefs B) fm (def_funs B B rhoc rhoc)
+      | S k => fun_map_inv' k (occurs_free_in_env rho1) fm (def_funs B B rhoc rhoc) rho2 i sig
       end.
 
-  Definition fun_map_inv (k : nat) (S : Ensemble var) (fm : fun_map) (rho : env) : Prop :=
+  Definition fun_map_inv (k : nat) (S : Ensemble var) (fm : fun_map) (rho1 rho2 : env) (i : nat) (sig : subst) : Prop :=
     forall f ft xs e rhoc B f',
       f \in S ->
       fm ! f = Some (ft, xs, e) ->
-      rho ! f = Some (Vfun rhoc B f') ->
+      rho1 ! f = Some (Vfun rhoc B f') ->
       find_def f B = Some (ft, xs, e) /\ f = f' /\
-      eq_env_P (occurs_free_fundefs B) rho rhoc /\      
+      preord_env_P_inj cenv PG (name_in_fundefs B :|: occurs_free_fundefs B) i (apply_r sig) (def_funs B B rhoc rhoc) rho2 /\
+      sub_map (def_funs B B rhoc rhoc) rho1 /\
+      Disjoint _ (bound_var e) (name_in_fundefs B :|: FromList xs :|: occurs_free_in_env rho1 :|: Dom_map rhoc) /\
+      Disjoint _ (FromList xs) (name_in_fundefs B :|: occurs_free_in_env rho1 :|: Dom_map rhoc :|: Dom_map fm) /\
       match k with
       | 0%nat => True
-      | S k => fun_map_inv' k (occurs_free_fundefs B) fm (def_funs B B rhoc rhoc)
+      | S k => fun_map_inv' k (occurs_free_in_env rho1) fm (def_funs B B rhoc rhoc) rho2 i sig
       end.
-    
-  Lemma fun_map_inv_eq k fm rho :
-    fun_map_inv k fm rho = fun_map_inv' k fm rho.
+
+  Lemma fun_map_inv_eq k S fm rho1 rho2 n sig :
+    fun_map_inv k S fm rho1 rho2 n sig = fun_map_inv' k S fm rho1 rho2 n sig.
   Proof.
     destruct k; reflexivity.
   Qed.
   
-  Lemma fun_map_inv_mon k k' S fm rho :
-    fun_map_inv k S fm rho ->
+  Lemma fun_map_inv_mon k k' S fm rho1 rho2 i sig :
+    fun_map_inv k S fm rho1 rho2 i sig ->
     (k' <= k)%nat ->
-    fun_map_inv k' S fm rho.
+    fun_map_inv k' S fm rho1 rho2 i sig.
   Proof.
-    revert S k fm rho. induction k' as [k' IHk] using lt_wf_rec1; intros.
+    revert S k fm rho1 rho2 i sig. induction k' as [k' IHk] using lt_wf_rec1; intros.
     destruct k'.
-    - unfold fun_map_inv in *. intros. edestruct H as [Hf [Heq [Heq' Hm]]]; eauto. 
+    - unfold fun_map_inv in *. intros. edestruct H; eauto. destructAll.
+      repeat (split; eauto).
     - destruct k; [ omega | ].
-      intro; intros. edestruct H as [Hf [Heq [Heq' Hm]]]; eauto. 
-      split; eauto. split; eauto. split; eauto. rewrite <- fun_map_inv_eq. eapply IHk. 
+      intro; intros. edestruct H; eauto. destructAll. 
+      split; eauto. split; eauto. split; eauto. split; eauto. split; eauto. split; eauto.
+      rewrite <- fun_map_inv_eq. eapply IHk. 
       omega. rewrite fun_map_inv_eq. eassumption. omega. 
   Qed.
-  
-  Lemma fun_map_inv_set k S fm rho x v :
-    fun_map_inv k S fm rho ->
-    ~ x \in Dom_map fm :|: occurs_free_in_env rho  ->
-    fun_map_inv k (x |: S) fm (M.set x v rho).           
+
+  Lemma fun_map_inv_i_mon k S fm rho1 rho2 i i' sig :
+    fun_map_inv k S fm rho1 rho2 i sig ->
+    (i' <= i)%nat ->
+    fun_map_inv k S fm rho1 rho2 i' sig.
   Proof.
-    intros Hinv Hnin. intro; intros.
-    rewrite M.gso in *.
-    2:{ intros Heq; subst. eapply Hnin. left. eexists; eauto. }
-    inv H.
-    - inv H2. exfalso. eapply Hnin. left. eexists; eauto.
-    - edestruct Hinv; eauto.
-      destructAll. split; [| split; [| split ]]; eauto.
-      eapply eq_env_P_set_not_in_P_l. eassumption.
-      intros Hc. eapply Hnin. right. do 4 eexists. split; eauto.    
+    revert k S fm rho1 rho2 i i' sig. induction k as [k' IHk] using lt_wf_rec1; intros.
+    intros. intro; intros. edestruct H; eauto. destructAll. split; eauto. split; eauto. split; eauto. 
+    eapply preord_env_P_inj_monotonic; eassumption.
+    split; eauto. split; eauto. split; eauto.
+    destruct k'; eauto. rewrite <- fun_map_inv_eq in *. eapply IHk; eauto.
   Qed.
 
-  (* Lemma occurs_free_in_env_set_compat rho rho' x v : *)
-  (*   occurs_free_in_env rho' \subset occurs_free_in_env rho -> *)
-  (*   occurs_free_in_env (M.set x v rho') \subset occurs_free_in_env (M.set x v rho). *)
-  (* Proof. *)
-  (*   intros Hc z [y Hin]. destructAll. *)
-  (*   destruct (peq x y); subst. *)
-  (*   - rewrite M.gss in H. inv H.  *)
-  (*     do 4 eexists; split; eauto. rewrite M.gss. reflexivity. *)
-  (*   - rewrite M.gso in H; eauto. edestruct Hc. now do 4 eexists; split; eauto. *)
-  (*     destructAll. do 4 eexists; split; eauto. rewrite M.gso. eassumption. reflexivity. *)
-  (*   rewrite M.gso. eassumption. *)
-  (*   intros Hd. eapply Hc. subst. eexists. eassumption. *)
-  (* Qed. *)
-      
+  Lemma fun_map_inv_antimon k S S' fm rho1 rho2 i sig :
+    fun_map_inv k S fm rho1 rho2 i sig ->
+    S' \subset S ->
+    fun_map_inv k S' fm rho1 rho2 i sig.
+  Proof.
+    intros H1 H2. intro; intros; eauto.
+  Qed.
+
+  Lemma sub_map_set {A} rho x (v : A) :
+    ~ x \in Dom_map rho ->
+    sub_map rho (M.set x v rho).
+  Proof.
+    intros Hnin z1 v1 Hget1. rewrite M.gso; eauto.
+    intros hc. subst. eapply Hnin. eexists; eauto.
+  Qed.
+
+  Lemma sub_map_trans {A} (rho1 rho2 rho3 : M.t A) :
+    sub_map rho1 rho2 ->
+    sub_map rho2 rho3 ->
+    sub_map rho1 rho3.
+  Proof.
+    intros H1 H2 x v Hget. eauto.
+  Qed.
+
+  Lemma sub_map_refl {A} (rho : M.t A) :
+    sub_map rho rho.
+  Proof.
+    intro; intros; eauto.
+  Qed.
+
   Lemma occurs_free_in_env_set rho x v :
     occurs_free_in_env (M.set x v rho) \subset occurs_free_in_val v :|: occurs_free_in_env rho.
   Proof.
@@ -330,6 +352,112 @@ Section Inline_correct.
     - rewrite M.gso in H; eauto. right.
       do 4 eexists; split; eauto.
   Qed.
+
+  Lemma occurs_free_in_env_get rho x v :
+    M.get x rho = Some v ->
+    occurs_free_in_val v \subset occurs_free_in_env rho.
+  Proof.
+    intros Hget z Hin.
+    destruct v; try now inv Hin.
+    do 4 eexists; split; eauto.
+  Qed.
+  
+  Lemma occurs_free_in_env_get_list (rho : env) xs vs :
+    get_list xs rho = Some vs ->
+    \bigcup_(v in FromList vs) (occurs_free_in_val v) \subset occurs_free_in_env rho.
+  Proof.
+    revert vs. induction xs; intros vs Hget.
+    - destruct vs; try now inv Hget. normalize_sets. rewrite big_cup_Empty_set. sets.
+    - simpl in Hget. destruct (rho!a) eqn:Hgeta; try now inv Hget.
+      destruct (get_list xs rho) eqn:Hgetl; try now inv Hget. inv Hget.
+      normalize_sets. rewrite Union_big_cup. rewrite big_cup_Singleton.
+      eapply Union_Included; eauto.
+      eapply occurs_free_in_env_get. eassumption.
+  Qed.
+
+  
+  Lemma occurs_free_in_env_def_funs B rho:
+    occurs_free_in_env (def_funs B B rho rho) \subset occurs_free_fundefs B :|: name_in_fundefs B :|: occurs_free_in_env rho.
+  Proof.
+    intros x1 Hin1. inv Hin1. destructAll.
+    destruct (Decidable_name_in_fundefs B). destruct (Dec x).
+    + rewrite def_funs_eq in H; eauto. inv H. now left; eauto.
+    + rewrite def_funs_neq in H; eauto. right. eapply occurs_free_in_env_get. eassumption.
+      eassumption.
+  Qed.
+  
+  Lemma occurs_free_in_env_def_funs' B rho:
+    occurs_free_fundefs B :|: name_in_fundefs B \subset occurs_free_in_env (def_funs B B rho rho).
+  Proof.
+    intros x Hc. destruct B.
+    - eapply occurs_free_in_env_get. simpl. rewrite M.gss. reflexivity. simpl. eassumption.
+    - inv Hc. inv H. inv H.
+  Qed.
+
+  Lemma sub_map_occurs_free_in_env rho1 rho2 :
+    sub_map rho1 rho2 ->
+    occurs_free_in_env rho1 \subset occurs_free_in_env rho2.
+  Proof.
+    intros Hs z Hin. inv Hin. destructAll.
+    eapply Hs in H. do 4 eexists. split. eassumption. eassumption.
+  Qed.
+
+  Lemma fun_map_inv_set_not_In_r k S fm rho1 rho2 i sig x x' v' : 
+    fun_map_inv k S fm rho1 rho2 i sig ->
+    ~ x \in occurs_free_in_env rho1 ->
+    ~ x' \in image (apply_r sig) (occurs_free_in_env rho1) ->
+    fun_map_inv k S fm rho1 (M.set x' v' rho2) i (M.set x x' sig).
+  Proof.
+    revert S fm rho1 rho2 i sig x x' v'. induction k using lt_wf_rec1; intros. intro; intros.
+    edestruct H0; eauto.
+    destructAll. split; [| split; [| split; [| split; [| split; [| split ]]]]]; eauto.
+    - rewrite apply_r_set_f_eq. eapply preord_env_P_inj_set_extend_not_In_P_r. eassumption.
+      + intros Hc. eapply H1.   
+        eapply occurs_free_in_env_get. eassumption. simpl. now inv Hc; eauto.
+      + intros Hc. eapply H2. eapply image_monotonic; [| eassumption ]. 
+        eapply Included_trans; [| eapply occurs_free_in_env_get; eauto ]. simpl. sets.
+    - destruct k; eauto. rewrite <- fun_map_inv_eq in *. eapply H. omega. eassumption.
+      + intros Hc. eapply H1.
+        eapply sub_map_occurs_free_in_env. eassumption. eassumption.
+      + intros Hc. eapply H2. eapply image_monotonic; [| eassumption ].
+        eapply sub_map_occurs_free_in_env. eassumption.
+  Qed.                
+    
+  Lemma fun_map_inv_set k S fm rho1 rho2 i sig x v x' v' :
+    fun_map_inv k S fm rho1 rho2 i sig ->
+    ~ x \in Dom_map rho1 :|: Dom_map fm :|: occurs_free_in_env rho1 ->
+    ~ x' \in image (apply_r sig) (occurs_free_in_env rho1) ->
+    occurs_free_in_val v \subset occurs_free_in_env rho1 ->
+    fun_map_inv k (x |: S) fm (M.set x v rho1) (M.set x' v' rho2) i (M.set x x' sig).
+  Proof.
+    intros Hinv Hnin Hnin' Hsub. intro; intros.
+    rewrite M.gso in *.
+    2:{ intros Heq; subst. eapply Hnin. left. right. eexists; eauto. }
+    inv H.
+    - inv H2. exfalso. eapply Hnin. left. left. eexists; eauto.
+    - edestruct Hinv; eauto.
+      destructAll. split; [| split; [| split; [| split; [| split; [| split ]]]]]; eauto.
+      + rewrite apply_r_set_f_eq. eapply preord_env_P_inj_set_extend_not_In_P_r. eassumption.
+        intros Hc. eapply Hnin.  
+        right. eapply occurs_free_in_env_get. eassumption. simpl. now inv Hc; eauto.
+        intros Hc. eapply Hnin'. eapply image_monotonic; [| eassumption ]. 
+        eapply Included_trans; [| eapply occurs_free_in_env_get; eauto ]. simpl. sets.
+      + eapply sub_map_trans. eassumption. eapply sub_map_set.
+        intros Hc. eapply Hnin. left. left. eassumption.
+      + eapply Union_Disjoint_r; [| now sets ].
+        eapply Union_Disjoint_r; [ now sets | ]. eapply Disjoint_Included_r. eapply occurs_free_in_env_set.
+        rewrite Union_Same_set. sets. eassumption. 
+      + eapply Union_Disjoint_r; [| now sets ]. eapply Union_Disjoint_r; [| now sets ].
+        eapply Union_Disjoint_r; [ now sets | ]. eapply Disjoint_Included_r. eapply occurs_free_in_env_set.
+        rewrite Union_Same_set. sets. eassumption.         
+      + destruct k; eauto. rewrite <- fun_map_inv_eq in *.
+        eapply fun_map_inv_set_not_In_r. eapply fun_map_inv_antimon. eassumption.
+        * eapply Included_trans. eapply occurs_free_in_env_set. sets.
+        * intros Hc. eapply Hnin. right. eapply sub_map_occurs_free_in_env; eassumption.
+        * intros Hc. eapply Hnin'. eapply image_monotonic; [| eassumption ].
+          eapply sub_map_occurs_free_in_env; eassumption.
+  Qed.
+  
 
   Lemma occurs_free_in_env_set_lists_not_In rho rho' xs vs :
     set_lists xs vs rho = Some rho' ->
@@ -344,32 +472,126 @@ Section Inline_correct.
       eauto.
   Qed.
 
-  Instance fm_map_Proper k : Proper (Same_set _ ==> eq ==> eq ==> iff) (fun_map_inv k).
+  Instance fm_map_Proper k : Proper (Same_set _ ==> eq ==> eq ==> eq ==> eq ==> eq ==> iff) (fun_map_inv k).
   Proof.
     repeat (intro; intros). subst. split; intros.
     intro; intros. rewrite <- H in H1. eauto.
     intro; intros. rewrite H in H1. eauto.
   Qed.
-  
-  Lemma fun_map_inv_set_lists k S fm rho rho' xs vs :
-    fun_map_inv k S fm rho ->
-    \bigcup_(v in FromList vs) (occurs_free_in_val v) \subset occurs_free_in_env rho ->
-    Disjoint _ (FromList xs) (Dom_map fm :|: occurs_free_in_env rho) ->
+
+  Lemma Dom_map_set_lists {A} xs (vs : list A) rho rho' :
     set_lists xs vs rho = Some rho' ->
-    fun_map_inv k (FromList xs :|: S) fm rho'.
+    Dom_map rho' <--> FromList xs :|: Dom_map rho.
   Proof.
-    revert S rho rho' vs; induction xs; intros S rho rho' vs Hfm Hs Hdis Hset.
-    - destruct vs; inv Hset; eauto. repeat normalize_sets. eauto.
-    - destruct vs; try now inv Hset. simpl in Hset.
-      destruct (set_lists xs vs rho) eqn:Hset'; inv Hset.
-      repeat normalize_sets. rewrite <- Union_assoc. eapply fun_map_inv_set.
-      eapply IHxs; eauto.
-      + eapply Included_trans; [| eassumption ]. eapply Included_big_cup. reflexivity.
-        sets.
-      + sets.
-      + intros Hc. eapply Hdis. constructor. now left. inv Hc; eauto.
-        eapply occurs_free_in_env_set_lists_not_In in H; [| now eauto ]. inv H; eauto.
-        right. eapply Hs. eapply Included_big_cup; [| | eassumption ]. reflexivity. sets.
+    revert vs rho'. induction xs; intros vs rho' Hset.
+    - destruct vs; inv Hset. repeat normalize_sets. reflexivity.
+    - destruct vs; try now inv Hset.
+      simpl in Hset. destruct (set_lists xs vs rho) eqn:Hset1; inv Hset.
+      repeat normalize_sets. rewrite Dom_map_set. rewrite IHxs. now sets.
+      eassumption.
+  Qed.
+
+  Lemma sub_map_set_lists {A} rho rho' xs (vs : list A) :
+    set_lists xs vs rho = Some rho' ->
+    NoDup xs ->
+    Disjoint _ (FromList xs) (Dom_map rho) ->
+    sub_map rho rho'.
+  Proof.
+    revert rho rho' vs; induction xs; intros rho rho' vs Hset; destruct vs; try now inv Hset.
+    simpl in Hset. destruct (set_lists xs vs rho) eqn:Hset'; inv Hset.
+    intros Hnd Hdis. inv Hnd. repeat normalize_sets. eapply sub_map_trans. eapply IHxs. eassumption. eassumption.
+    now sets. eapply sub_map_set. intros Hc. eapply Hdis. constructor. now left.
+    eapply Dom_map_set_lists in Hc; eauto. inv Hc; eauto. exfalso. contradiction.
+  Qed.
+
+  Lemma apply_r_set_list_f_eq xs ys sig : 
+    f_eq (apply_r (set_list (combine xs ys) sig)) (apply_r sig <{ xs ~> ys }>). 
+  Proof.
+    revert ys sig. induction xs; intros; simpl. reflexivity.
+    destruct ys. reflexivity.
+    simpl. eapply Equivalence_Transitive.
+    eapply apply_r_set_f_eq. eapply f_eq_extend. eauto.
+  Qed.
+
+
+  Lemma fun_map_inv_sig_extend_Disjoint k S fm rho1 rho2 i sig xs xs' :
+    fun_map_inv k S fm rho1 rho2 i sig ->
+
+    Disjoint _ (FromList xs) (S :|: occurs_free_in_env rho1) ->    
+    
+    fun_map_inv k S fm rho1 rho2 i (set_list (combine xs xs') sig).
+  Proof.
+    revert S fm rho1 rho2 i sig xs xs'.
+    induction k using lt_wf_rec1; intros S fm rho1 rho2 i sig xs xs' Hfm Hdis1.
+    intro; intros. edestruct Hfm; eauto. destructAll.
+    split; eauto. split; eauto. split; [| split; [| split; [| split ]]].
+    - rewrite apply_r_set_list_f_eq. 
+      eapply preord_env_P_inj_extend_lst_not_In_P_r. eassumption.
+      eapply Disjoint_Included_r; [| eapply Hdis1 ].
+      eapply Included_Union_preserv_r. eapply Included_trans; [| eapply occurs_free_in_env_get; eauto ].
+      simpl; now sets.
+    - eassumption.
+    - eassumption.
+    - eassumption.
+    - destruct k; eauto. rewrite <- fun_map_inv_eq in *. eapply H. omega.
+      eassumption.
+      eapply Disjoint_Included_r; [| eassumption ].
+      eapply Included_Union_preserv_r. eapply Union_Included.
+      + reflexivity.
+      + eapply sub_map_occurs_free_in_env. eassumption.
+  Qed.
+
+  Lemma fun_map_inv_set_lists k S S' fm rho1 rho1' rho2 rho3 i sig xs xs' vs :
+    fun_map_inv k S fm rho1 rho2 i sig ->
+
+    fun_map_inv k S' fm rho3 rho2 i sig ->
+    S \subset S' ->
+    \bigcup_(v in FromList vs) occurs_free_in_val v \subset occurs_free_in_env rho3 ->
+    sub_map rho1 rho3 ->
+    
+    NoDup xs ->
+    Disjoint _ (FromList xs) (Dom_map rho1 :|: Dom_map fm :|: occurs_free_in_env rho3) ->    
+    set_lists xs vs rho1 = Some rho1' ->
+    
+    fun_map_inv k (FromList xs :|: S) fm rho1' rho2 i (set_list (combine xs xs') sig).
+  Proof.
+    revert S S' fm rho1 rho1' rho2 rho3 i sig xs xs' vs.
+    induction k using lt_wf_rec1;
+      intros S S' fm rho1 rho1' rho3 rho2 i sig xs xs' vs Hfm Hfm' Hsub Hsub' Hsm Hnd Hdis1 Hset.
+    intro; intros.
+    destruct (Decidable_FromList xs). destruct (Dec f).
+    - exfalso. eapply Hdis1. constructor. eassumption. left. right. eexists; eauto.
+    - inv H0; try contradiction. erewrite <- set_lists_not_In in H2; [| eassumption | eassumption ].
+      edestruct Hfm; eauto. destructAll. split; eauto. split; eauto. split; [| split; [| split; [| split ]]].
+      + rewrite apply_r_set_list_f_eq. 
+        eapply preord_env_P_inj_extend_lst_not_In_P_r. eassumption.
+        eapply Disjoint_Included_r; [| eapply Hdis1 ].
+        eapply Included_Union_preserv_r. eapply Included_trans; [| eapply occurs_free_in_env_get; eauto ].
+        simpl; now sets.
+      + eapply sub_map_trans. eassumption. eapply sub_map_set_lists. eassumption. eassumption.
+        eapply Disjoint_Included_r; [| eapply Hdis1 ]. sets.
+      + edestruct Hfm'. eapply Hsub. eassumption. eassumption. eapply Hsm. eassumption.
+        destructAll.
+        eapply Union_Disjoint_r; [| now sets ]. eapply Union_Disjoint_r; [ now sets | ].
+        eapply Disjoint_Included_r. eapply occurs_free_in_env_set_lists_not_In. eassumption.
+        eapply Union_Disjoint_r; [| eapply Disjoint_Included_r; [| eapply H7]; now sets ].
+        eapply Disjoint_Included_r. eassumption. sets.
+      + edestruct Hfm'. eapply Hsub. eassumption. eassumption. eapply Hsm. eassumption.
+        destructAll.
+        eapply Union_Disjoint_r; [| now sets ]. eapply Union_Disjoint_r; [| now sets ]. eapply Union_Disjoint_r; [ now sets | ].
+        eapply Disjoint_Included_r. eapply occurs_free_in_env_set_lists_not_In. eassumption.
+        eapply Union_Disjoint_r; sets. eapply Disjoint_Included_r; [| eapply H8 ]. sets.
+      + destruct k; eauto.
+        edestruct Hfm'. now eauto. eassumption. eapply Hsm. eassumption. destructAll. 
+        rewrite <- fun_map_inv_eq in *. eapply fun_map_inv_sig_extend_Disjoint.
+        eapply fun_map_inv_antimon. eapply H15.
+        eapply Included_trans. eapply occurs_free_in_env_set_lists_not_In. eassumption.
+        eapply Union_Included. eassumption. eapply sub_map_occurs_free_in_env. eassumption.
+        eapply Disjoint_Included_r; [| eassumption ].
+        eapply Included_Union_preserv_r. eapply Union_Included.
+        * eapply Included_trans. eapply occurs_free_in_env_set_lists_not_In. eassumption.
+          eapply Union_Included. eassumption. eapply sub_map_occurs_free_in_env. eassumption.
+        * eapply sub_map_occurs_free_in_env. eassumption.
   Qed.
   
   Lemma add_fundefs_in fm f B ft xs e:
@@ -401,203 +623,152 @@ Section Inline_correct.
     rewrite Dom_map_set. rewrite IHB. sets.
   Qed.
 
-  Lemma fun_map_inv_def_funs k fm rho B :
-    fun_map_inv k fm rho ->
-    Disjoint _ (name_in_fundefs B) (fun_bindings_env rho) ->
-    fun_map_inv k (add_fundefs B fm) (def_funs B B rho rho).
+(* 
+    
+  Lemma fun_map_inv_add_fundefs_Disjoint k S fm rho1 rho2 i sig B :
+    fun_map_inv k S fm rho1 rho2 i sig ->
+    Disjoint _ (name_in_fundefs B) (S :|: occurs_free_in_env rho1) ->
+    fun_map_inv k S (add_fundefs B fm) rho1 rho2 i sig.
   Proof.
-    revert fm rho B. induction k as [k IHk] using lt_wf_rec1. intros fm rho B Hf Hdis.
-    intros f ft xs e rhoc B' f' Heq1 Heq2.  
-    destruct (Decidable_name_in_fundefs B) as [Dec]. destruct (Dec f).
+    revert S fm rho1 rho2 i sig  B; induction k using lt_wf_rec1; intros.
+    intro; intros. rewrite add_fundefs_not_in in H3.
+    edestruct H0; eauto. destructAll.
+    repeat (split; [ now eauto |]). split.
+    - rewrite Dom_map_add_fundefs. sets. 
+      reflexivity. split. eassumption. split. eassumption.
+    destruct k; eauto. rewrite <- fun_map_inv_eq in *. eapply H.
+    + omega.
+    + eassumption.
+    + eapply Disjoint_Included_r; [| eassumption ].
+      eapply Included_Union_preserv_r. eapply Union_Included.
+      * eapply Included_trans; [| eapply occurs_free_in_env_get ]; eauto.
+        simpl; sets.
+      * eapply sub_map_occurs_free_in_env. eassumption.
+    + intros Hc. eapply H1. constructor. eassumption. now left.
+  Qed.
+
+  Lemma sub_map_def_funs rho B :
+    Disjoint _ (name_in_fundefs B) (Dom_map rho) ->            
+    sub_map rho (def_funs B B rho rho).
+  Proof.
+    intros Hdis x v Hget.
+    rewrite def_funs_neq; eauto.
+    intros Hc. eapply Hdis. constructor. eassumption. eexists. eassumption.
+  Qed.    
+
+  Lemma fun_map_inv_def_funs k S fm rho1 rho2 i sig B1 B2 :
+    fun_map_inv k S fm rho1 rho2 i sig ->
+    preord_env_P_inj cenv PG (name_in_fundefs B1 :|: occurs_free_fundefs B1) i
+                     (apply_r (set_list (combine (all_fun_name B1) (all_fun_name B2)) sig))
+                     (def_funs B1 B1 rho1 rho1) (def_funs B2 B2 rho2 rho2) ->
+    occurs_free_fundefs B1 \subset S ->
+    Disjoint _ (name_in_fundefs B1) (S :|: Dom_map rho1 :|: occurs_free_in_env rho1) ->
+
+    fun_map_inv k (name_in_fundefs B1 :|: S) (add_fundefs B1 fm) (def_funs B1 B1 rho1 rho1) (def_funs B2 B2 rho2 rho2) i
+                (set_list (combine (all_fun_name B1) (all_fun_name B2)) sig).
+  Proof.
+    revert S fm rho1 rho2 i sig B1 B2. induction k as [k IHk] using lt_wf_rec1. intros S fm rho1 rho2 i sig B1 B2 Hf Hrel Hsub Hdis.
+    intros f ft xs e rhoc B' f' HSin Heq1 Heq2.   
+    destruct (Decidable_name_in_fundefs B1) as [Dec]. destruct (Dec f).
     - rewrite def_funs_eq in Heq2; eauto. inv Heq2.
       edestruct name_in_fundefs_find_def_is_Some. eassumption. destructAll.
       erewrite add_fundefs_in in Heq1; [| eassumption ]. inv Heq1. split; eauto.
-      split; eauto. destruct k; eauto. rewrite <- fun_map_inv_eq. eapply IHk. omega.
-      eapply fun_map_inv_mon. eassumption. omega.
-      eassumption.
+      split; eauto. split; [| split ].
+      + eassumption.
+      + eapply sub_map_refl.
+      + destruct k; eauto. rewrite <- fun_map_inv_eq. eapply IHk. omega.
+        eapply fun_map_inv_antimon. eapply fun_map_inv_mon. eassumption. omega.
+        eassumption. eassumption. reflexivity. eapply Disjoint_Included_r; [| eassumption ].
+        eapply Union_Included; sets.
     - rewrite def_funs_neq in Heq2; eauto.
-      rewrite add_fundefs_not_in in Heq1; [| eassumption ].
-      edestruct Hf. eassumption. eassumption. destructAll. split; eauto. split; eauto. 
-      destruct k; eauto. rewrite <- fun_map_inv_eq in *.
-      assert (Hdis' : Disjoint _ (name_in_fundefs B) (name_in_fundefs B' :|: funs_in_env rhoc)).
-      { eapply Disjoint_Included_r; [| eassumption ].
-        eapply Included_trans; [| eapply fun_bindings_env_get ]; [| eassumption ].
-        reflexivity. }      
-      clear Dec H Hf Heq2 Hdis. 
-      revert rhoc B' B n H1 Hdis'. induction k as [k IHk2] using lt_wf_rec1; intros.
-      intro; intros.
-      rewrite add_fundefs_not_in in H; eauto. 
-      edestruct H1. eassumption. eassumption. destructAll. split; eauto. split; eauto.
-      destruct k; eauto. rewrite <- fun_map_inv_eq in *. 
-      eapply IHk2. omega. now eauto. eassumption. eassumption. admit. eassumption. 
-      { intros Hc.
-        eapply Hdis. constructor. eassumption. SearchAbout rho.
-        destruct (Decidable_name_in_fundefs B') as [Dec]. destruct (Dec f).
-        
-
-        intros Hin. eapply Hdis. constructor. eassumption. eapply H1. eassumption.
-  Qed.
-
-(*   
-  Definition fun_map_inv (fm : fun_map) (rho : env) (* (sig : subst) *) :=
+      rewrite add_fundefs_not_in in Heq1; [| eassumption ]. inv HSin. contradiction. 
+      edestruct Hf. eassumption. eassumption. eassumption. destructAll. split; eauto. split; eauto. 
+      split; [| split ].
+      + admit.
+        (* eapply eq_env_P_def_funs_not_in_P_r. eassumption. *)
+        (* eapply Disjoint_sym. eapply Disjoint_Included_r; [| eassumption ]. *)
+        (* eapply Included_Union_preserv_r. *)
+        (* eapply Included_trans; [| eapply occurs_free_in_env_get ]; eauto. simpl. sets. *)
+      + eapply sub_map_trans. eassumption. eapply sub_map_def_funs. sets.
+      + destruct k; eauto. rewrite <- fun_map_inv_eq in *.
+        eapply fun_map_inv_add_fundefs_Disjoint. admit.
+        (* eassumption. *)
+  (*       eapply Disjoint_Included_r; [| eassumption ]. eapply Included_Union_preserv_r. *)
+  (*       eapply Union_Included. *)
+  (*       eapply Included_trans; [| eapply occurs_free_in_env_get ]; eauto. simpl; now sets. *)
+  (*       eapply sub_map_occurs_free_in_env. eassumption. *)
+  (* Qed. *)
+  Abort.
+ *)
+  
+  Definition fun_map_vars (fm : fun_map) (F : Ensemble var) (sig : subst) :=
     forall f ft xs e,
       fm ! f = Some (ft, xs, e) ->
-      exists rhoc B, rho ! f = Some (Vfun rhoc B f) /\
-                     find_def f B = Some (ft, xs, e) /\
-                     (forall g, g \in name_in_fundefs B ->
-                                rho ! g = Some (Vfun rhoc B g) /\ g \in Dom_map fm).
-  
-  Lemma fun_map_inv_set fm rho x v :
-    fun_map_inv fm rho ->
-    ~ x \in Dom_map fm ->
-    fun_map_inv fm (M.set x v rho).           
+      unique_bindings e /\
+      NoDup xs /\
+      Disjoint _ (bound_var e) (occurs_free e :|: Dom_map fm) /\
+      Disjoint _ F (bound_var e :|: image (apply_r sig) (occurs_free e)).
+
+  Definition occurs_free_fun_map (fm : fun_map) : Ensemble var :=
+    fun v => exists f ft xs e, fm ! f = Some (ft, xs, e) /\ v \in (occurs_free e \\ FromList xs).
+
+  Lemma fun_map_vars_set fm F sig x v :
+    fun_map_vars fm F sig ->
+    fun_map_vars fm (F \\ [set v]) (M.set x v sig).
   Proof.
-    intros Hinv Hnin f ft xs e Hget.
-    rewrite M.gso.
-    - eapply Hinv in Hget. destructAll. do 2 eexists. split; eauto. split; eauto.
-      intros. rewrite M.gso. eauto. intro; subst. eapply H1 in H2.
-      inv H2. contradiction.
-    - intros Heq; subst. eapply Hnin.
-      eexists; eauto.
-  Qed.
-    
-  Lemma fun_map_inv_set_lists fm rho rho' xs vs :
-    fun_map_inv fm rho ->
-    Disjoint _ (FromList xs) (Dom_map fm) ->
-    set_lists xs vs rho = Some rho' ->
-    fun_map_inv fm rho'.
-  Proof.
-    revert rho rho' vs; induction xs; intros rho rho' vs Hfm Hdis Hset.
-    - destruct vs; inv Hset; eauto.
-    - destruct vs; try now inv Hset. simpl in Hset.
-      destruct (set_lists xs vs rho) eqn:Hset'; inv Hset.
-      repeat normalize_sets.
-      eapply fun_map_inv_set. eapply IHxs; eauto.
-      now sets. intros Hc. eapply Hdis. constructor. now left.
-      eassumption.
-  Qed.
-  
-  Lemma add_fundefs_in fm f B ft xs e:
-    find_def f B = Some (ft, xs, e) -> 
-    (add_fundefs B fm) ! f = Some (ft, xs, e). 
-  Proof.
-    induction B.
-    - simpl. intros Hdef. destruct (M.elt_eq f v); subst.
-      + inv Hdef. simpl. rewrite M.gss. reflexivity.
-      + simpl. rewrite M.gso; eauto.
-    - intros H. inv H.
+    intros Hfm; intro; intros. eapply Hfm in H. destructAll.
+    do 3 (split; eauto). eapply Union_Disjoint_r. now sets.
+    eapply Disjoint_Included_r. eapply image_apply_r_set.
+    eapply Union_Disjoint_r. now sets. now xsets.
   Qed.
 
-  Lemma add_fundefs_not_in fm f B :
-    ~ f \in name_in_fundefs B -> 
-    (add_fundefs B fm) ! f = fm ! f.
+  Lemma Dom_map_def_funs B rho B' rho' :
+    Dom_map (def_funs B' B rho' rho) <--> name_in_fundefs B :|: Dom_map rho. 
   Proof.
-    intros Hnin. induction B.
-    - simpl. rewrite M.gso. eapply IHB.
-      intros Hc. eapply Hnin. simpl. now right; eauto.
-      intros Hc. eapply Hnin. simpl. subst; eauto.
-    - reflexivity.
-  Qed.
-
-  Lemma Dom_map_add_fundefs fm B :
-    Dom_map (add_fundefs B fm) <--> name_in_fundefs B :|: Dom_map fm.
-  Proof.
-    induction B; simpl; [| now sets ].
+    induction B; simpl; sets.
     rewrite Dom_map_set. rewrite IHB. sets.
   Qed.
-
-  Lemma fun_map_inv_def_funs fm rho B :
-    fun_map_inv fm rho ->
-    Disjoint _ (name_in_fundefs B) (Dom_map fm) ->
-    fun_map_inv (add_fundefs B fm) (def_funs B B rho rho).
-  Proof.
-    intros Hf Hd. intros f ft xs e Hget.
-    destruct (Decidable_name_in_fundefs B) as [Dec]. destruct (Dec f).
-    - do 2 eexists. split; [| split; [| split ]].
-      + eapply def_funs_eq in n. eassumption.
-      + edestruct name_in_fundefs_find_def_is_Some. eassumption.
-        destructAll. rewrite H. eapply add_fundefs_in in H. rewrite H in Hget.
-        inv Hget. reflexivity.
-      + rewrite def_funs_eq. reflexivity. eassumption.
-      + rewrite Dom_map_add_fundefs. sets.
-    - rewrite add_fundefs_not_in in Hget; [| eassumption ]. rewrite def_funs_neq; eauto.
-      eapply Hf in Hget. destructAll. do 2 eexists. split; eauto. split; eauto.
-      intros. rewrite def_funs_neq; eauto. split; eauto. eapply H1. eassumption.
-      rewrite Dom_map_add_fundefs. right. eapply H1; eauto.
-      intros Hin. eapply Hd. constructor. eassumption. eapply H1. eassumption.
-  Qed.
-*)
-  (* Lemma fun_map_inv_redef_funs fm rho B ft xs e rhoc f  : *)
-  (*   fun_map_inv fm rho -> *)
-  (*   fm ! f = Some (ft, xs, e) -> *)
-  (*   rho ! f = Some (Vfun rhoc B f) -> *)
-  (*   fun_map_inv fm (def_funs B B rho rho). *)
-  (* Proof. *)
-  (*   intros Hf Hg1 Hg2. intros g ft' xs' e' Hget. *)
-  (*   destruct (Decidable_name_in_fundefs B) as [Dec]. destruct (Dec g). *)
-  (*   - assert (Hg1' := Hg1). eapply Hf in Hg1. destructAll.  *)
-  (*     rewrite Hg2 in H. inv H. erewrite def_funs_eq; eauto. *)
-  (*     do 2 eexists. split. reflexivity. *)
-  (*     eapply H1 in n. destructAll. destruct H2. destruct x1 as [[? ? ] ?]. rewrite Hget in H2; inv H2.  *)
-  (*     eapply Hf in Hget. destructAll. rewrite H2 in H. inv H. split. eassumption. *)
-  (*     intros. rewrite def_funs_eq; eauto. split. reflexivity. eapply H4. eassumption. *)
-  (*   - rewrite def_funs_neq; eauto. *)
-  (*     eapply Hf in Hget. destructAll. do 2 eexists. split; eauto. split; eauto. *)
-
-  (*     intros g1 Hc. destruct (Decidable_name_in_fundefs B) as [Dec']. destruct (Dec' g1). clear Dec Dec'. *)
-  (*     + eapply Hf in Hg1. destructAll. repeat subst_exp.  *)
-  (*       eapply H4 in n0. destructAll.  *)
-  (*       eapply H1 in Hc. destructAll. repeat subst_exp.  *)
-  (*       rewrite def_funs_eq; eauto. *)
-        
-  (*       split. reflexivity. *)
-  (*     repeat subst_exp. do 10 subst_exp.  *)
-      (*   destruct (Decidable_name_in_fundefs B) as [Dec]. destruct (Dec f). *)
-  (*   - do 3 eexists. split. *)
-  (*     + eapply def_funs_eq in n. eassumption. *)
-  (*     + edestruct name_in_fundefs_find_def_is_Some. eassumption. *)
-  (*       destructAll. rewrite H. eapply add_fundefs_in in H. rewrite H in Hget. *)
-  (*       inv Hget. reflexivity. *)
-  (*   - rewrite add_fundefs_not_in in Hget; [| eassumption ]. rewrite def_funs_neq; eauto. *)
-  (* Qed. *)
-  (* Abort. *)
-  
+    
   Opaque preord_exp'.
   
   Lemma inline_correct d e sig fm st S :
     unique_bindings e ->
-    Disjoint _ (bound_var e) (occurs_free e) ->
+    Disjoint _ (bound_var e) (occurs_free e :|: Dom_map fm) ->    
     Disjoint _ S (bound_var e :|: image (apply_r sig) (occurs_free e)) ->
-    Disjoint _ (Dom_map fm) (bound_var e) ->       
+
+    fun_map_vars fm S sig ->
+    
     {{ fun _ s => fresh S (next_var (fst s)) }}
       beta_contract St IH d e sig fm st
     {{ fun _ _ e' s' =>
          fresh S (next_var (fst s')) /\
          (* unique bindings is preserved *)
          unique_bindings e' /\
-         occurs_free e' \subset image (apply_r sig) (occurs_free e) /\
+         occurs_free e' \subset image (apply_r sig) (occurs_free e :|: occurs_free_fun_map fm) /\
          bound_var e' \subset S /\
          (* Disjointedness is preserved *)
          (* Disjoint _ (bound_var e') (occurs_free e') /\ *)
          (* FV are preserved *)
          (* semantics are preserved *)
-         (forall rho1 rho2 k,
+         (forall k rho1 rho2,
              preord_env_P_inj cenv PG (occurs_free e) k (apply_r sig) rho1 rho2 ->
-             fun_map_inv fm rho1 ->
+             Disjoint _ (bound_var e) (occurs_free_in_env rho1 :|: Dom_map rho1) ->
+             fun_map_inv d (occurs_free e :|: occurs_free_in_env rho1) fm rho1 rho2 k sig ->
              preord_exp cenv P1 PG k (e, rho1) (e', rho2))
 
     }}.
   Proof.
     revert e sig fm st S. induction d as [d IHd] using lt_wf_rec1.
-    induction e using exp_ind'; intros sig fm st S Hun Hdis1 Hdis2 Hdis3; inv Hun; rewrite beta_contract_eq.
+    induction e using exp_ind'; intros sig fm st S Hun Hdis1 Hdis2 Hfm; inv Hun; rewrite beta_contract_eq.
     - (* constr *)
       eapply bind_triple. now eapply get_name_fresh. 
       intros x w1. eapply pre_curry_l. intros Hinx.
       eapply bind_triple. eapply IHe with (S := S \\ [set x]).
-      + eassumption. 
+      + eassumption.
       + repeat normalize_bound_var_in_ctx. repeat normalize_occurs_free_in_ctx.
         eapply Disjoint_Included_r. eapply Included_Union_Setminus with (s2 := [set v]). tci.
-        eapply Union_Disjoint_r. eapply Disjoint_Included; [| | eapply Hdis1]; now sets.
+        eapply Union_Disjoint_r. eapply Disjoint_Included; [| | eapply Hdis1].
+        rewrite Setminus_Union_distr. now sets. now sets.
         eapply Disjoint_Singleton_r. eassumption.
       + eapply Disjoint_Included_r.
         eapply Included_Union_compat. reflexivity.
@@ -607,22 +778,24 @@ Section Inline_correct.
         eapply Union_Disjoint_r. now sets.
         eapply Disjoint_Included; [| | eapply Hdis2 ]. rewrite image_Union. now sets.
         now sets.
-      + repeat normalize_bound_var_in_ctx. sets.
+      + eapply fun_map_vars_set. eassumption.
       + intros e' w2. eapply return_triple.
         intros _ st'. intros [Hf [Hun [Hsub [Hsub' Hsem]]]].
         split; [| split; [| split; [| split ]]].
         * eapply fresh_monotonic;[| eassumption ]. sets.
         * constructor.
           intros Hc. eapply Hsub' in Hc. now inv Hc; eauto. eassumption. 
-        * repeat normalize_occurs_free. rewrite image_Union.
-          rewrite <- FromList_apply_list. eapply Included_Union_compat. reflexivity. 
+        * repeat normalize_occurs_free. rewrite !image_Union.
+          rewrite <- FromList_apply_list. rewrite <- !Union_assoc. eapply Included_Union_compat. reflexivity. 
           eapply Included_trans. eapply Included_Setminus_compat.
           eapply Included_trans. eassumption. now eapply image_apply_r_set. reflexivity.
-          rewrite Setminus_Union_distr. rewrite Setminus_Same_set_Empty_set. normalize_sets. sets.
+          rewrite !Setminus_Union_distr. rewrite Setminus_Same_set_Empty_set. normalize_sets.
+          rewrite image_Union. sets.
         * normalize_bound_var. eapply Union_Included. eapply Included_trans. eassumption. now sets.
           eapply Singleton_Included. eassumption.
-        * intros r1 r2 k Henv Hfm. eapply preord_exp_const_compat.
-          admit. admit. admit.
+        * intros r1 r2 k Henv Hdis Hfm'. eapply preord_exp_const_compat.
+          eassumption. eassumption.
+          eapply Forall2_preord_var_env_map. eassumption. normalize_occurs_free. now sets.          
           intros. eapply Hsem. 
           rewrite apply_r_set_f_eq. eapply preord_env_P_inj_set_alt.
           -- eapply preord_env_P_inj_antimon. eapply preord_env_P_inj_monotonic; [| eassumption ].
@@ -631,8 +804,23 @@ Section Inline_correct.
              eapply Forall2_Forall2_asym_included. eassumption.
           -- intros Hc. eapply Hdis2. constructor. eassumption.
              right. normalize_occurs_free. rewrite image_Union. right. eassumption.
-          -- eapply fun_map_inv_set. eassumption.
-             eapply Disjoint_Singleton_In. tci. repeat normalize_bound_var_in_ctx. sets.
+          -- repeat normalize_bound_var_in_ctx. rewrite Dom_map_set.
+             eapply Union_Disjoint_r.
+             ++ eapply Disjoint_Included_r. eapply occurs_free_in_env_set. simpl. normalize_sets.
+                eapply Disjoint_Included; [| | eapply Hdis]; sets.
+             ++ eapply Union_Disjoint_r.
+                ** eapply Disjoint_Singleton_r. eassumption.
+                ** eapply Disjoint_Included; [| | eapply Hdis]; sets.
+          -- eapply fun_map_inv_antimon. eapply fun_map_inv_set. eapply fun_map_inv_i_mon. eassumption. omega.
+             intros Hc. inv Hc. inv H2.
+             ++ eapply Hdis. normalize_bound_var. constructor. now right. now right; eauto.
+             ++ eapply Hdis1. constructor. normalize_bound_var. now right. now right; eauto.
+             ++ eapply Hdis. normalize_bound_var. constructor. now right. now left; eauto.
+             ++ admit. (* change assumptions *)
+             ++ simpl. sets.
+             ++ normalize_occurs_free. rewrite !Union_assoc. rewrite Union_Setminus_Included; sets; tci.
+                eapply Union_Included. now sets. eapply Included_trans. eapply occurs_free_in_env_set.
+                simpl. sets.
     - (* Ecase [] *)
       admit.
     - (* Ecase (_ :: _) *)
@@ -651,40 +839,110 @@ Section Inline_correct.
           -- eapply return_triple.
              intros. split; [| split; [| split; [| split ]]]; try eassumption.
              ++ constructor.
-             ++ simpl. repeat normalize_occurs_free. rewrite image_Union, image_Singleton.
-                rewrite FromList_apply_list. reflexivity.
+             ++ simpl. repeat normalize_occurs_free. rewrite !image_Union, image_Singleton.
+                rewrite FromList_apply_list. sets.
+             ++ normalize_bound_var. sets.
+             ++ intros. eapply preord_exp_app_compat.
+                assumption. assumption.
+                eapply H0. now constructor.
+                eapply Forall2_preord_var_env_map. eassumption.
+                now constructor.              
+          -- destruct (Datatypes.length xs =? Datatypes.length l)%nat eqn:Hbeq.
+             { symmetry in Hbeq. eapply beq_nat_eq in Hbeq.
+               edestruct Hfm. eassumption. destructAll. eapply post_weakening; [| eapply IHd ].
+               ++ simpl. intros. destructAll. 
+                  split; [| split; [| split; [| split ]]]; try eassumption.
+                  ** eapply Included_trans. eassumption. 
+                     eapply Included_trans. eapply image_apply_r_set_list.
+                     unfold apply_r_list. rewrite list_length_map. eassumption.
+                     normalize_occurs_free. rewrite !image_Union. rewrite FromList_apply_list.
+                     eapply Union_Included. now sets.
+                     rewrite !Setminus_Union_distr. rewrite !image_Union. eapply Included_Union_preserv_r.
+                     eapply Union_Included; [| now sets ].
+                     eapply image_monotonic. intros z Hin. do 4 eexists; split; eauto.
+                  ** intros. eapply preord_exp_app_l.
+                   --- admit. (* post *)
+                   --- admit. (* post *)
+                   --- intros. assert (Hf := H11). assert (Heqf' := Heqf). edestruct H11; eauto. destructAll.
+                       do 2 subst_exp. eapply H8.
+                       +++ edestruct preord_env_P_inj_get_list_l. now eapply H9. normalize_occurs_free. now sets.
+                           eassumption. destructAll.                           
+                           eapply preord_env_P_inj_set_lists_l'; try eassumption. eapply preord_env_P_inj_antimon. eassumption.
+                           eapply Setminus_Included_Included_Union. eapply Included_trans. eapply occurs_free_in_fun.
+                           eapply find_def_correct. eassumption. sets.
+                       +++ erewrite Dom_map_set_lists; [| eassumption ]. rewrite Dom_map_def_funs.
+                           eapply Union_Disjoint_r; [| now xsets ].
+                           eapply Disjoint_Included_r. eapply occurs_free_in_env_set_lists_not_In. eassumption.
+                           eapply Disjoint_Included_r. eapply Included_Union_compat. reflexivity.
+                           eapply sub_map_occurs_free_in_env. eassumption.
+                           rewrite Union_Same_set. now sets. eapply occurs_free_in_env_get_list. eassumption. 
+                       +++  eapply fun_map_inv_antimon. eapply fun_map_inv_set_lists; [ | | | | | | | eassumption ].
+                            *** rewrite <- fun_map_inv_eq in *. eapply H22.
+                            *** eapply fun_map_inv_mon. eapply Hf. omega.
+                            *** sets.
+                            *** eapply occurs_free_in_env_get_list. eassumption.
+                            *** eassumption.
+                            *** eassumption. 
+                            *** rewrite Dom_map_def_funs. xsets.
+                            *** eapply Included_trans. eapply Included_Union_compat. reflexivity.
+                                eapply occurs_free_in_env_set_lists_not_In. eassumption.
+                                eapply Union_Included; [| eapply Union_Included ]. 
+                                ++++ eapply Included_trans.
+                                     2:{ eapply Included_Union_compat. reflexivity. eapply occurs_free_in_env_get. eapply H13. }
+                                     eapply Included_trans. eapply occurs_free_in_fun. eapply find_def_correct. eassumption.
+                                     sets.
+                                ++++ eapply Included_trans. eapply occurs_free_in_env_get_list. eassumption. sets.
+                                ++++ eapply Included_trans. eapply sub_map_occurs_free_in_env. eassumption. sets.
+               ++ omega.
+               ++ eassumption.
+               ++ eassumption.
+               ++ eapply Union_Disjoint_r. now sets.
+                  eapply Disjoint_Included_r. eapply image_apply_r_set_list.
+                  unfold apply_r_list. rewrite list_length_map. eassumption.
+                  eapply Union_Disjoint_r.
+                  eapply Disjoint_Included_r; [| eapply Hdis2 ]. normalize_occurs_free.
+                  rewrite image_Union. rewrite FromList_apply_list. now sets. now sets.
+               ++ (* Make lemma if needed about fun_map_vars fm S (set_list (combine xs (apply_r_list sig l)) sig) *)
+                  intros ? ? ? ? ?. edestruct Hfm; eauto. destructAll.
+                  repeat (split; [ now eauto |]). eapply Union_Disjoint_r. now sets.
+                  eapply Disjoint_Included_r. eapply image_apply_r_set_list.
+                  unfold apply_r_list. rewrite list_length_map. eassumption.
+                  eapply Union_Disjoint_r.
+                  eapply Disjoint_Included_r; [| eapply Hdis2 ]. normalize_occurs_free.
+                  rewrite image_Union. rewrite FromList_apply_list. now sets. now sets. }
+             { eapply return_triple.
+               intros. split; [| split; [| split; [| split ]]]; try eassumption.
+               ++ constructor.
+               ++ simpl. repeat normalize_occurs_free. rewrite !image_Union, image_Singleton.
+                  rewrite FromList_apply_list. sets.
+               ++ normalize_bound_var. sets.
+               ++ intros. eapply preord_exp_app_compat.
+                  assumption. assumption.
+                  eapply H0. now constructor.
+                  eapply Forall2_preord_var_env_map. eassumption.
+                  now constructor. }
+          -- eapply return_triple.
+             intros. split; [| split; [| split; [| split ]]]; try eassumption.
+             ++ constructor.
+             ++ simpl. repeat normalize_occurs_free. rewrite !image_Union, image_Singleton.
+                rewrite FromList_apply_list. sets.
              ++ normalize_bound_var. sets.
              ++ intros. eapply preord_exp_app_compat.
                 assumption. assumption.
                 eapply H0. now constructor.
                 eapply Forall2_preord_var_env_map. eassumption.
                 now constructor.
-          -- eapply post_weakening; [| eapply IHd ].
-             ++ simpl. intros. destructAll. 
-                split; [| split; [| split; [| split ]]]; try eassumption.
-                ** eapply Included_trans. eassumption.
-                   (* eapply Included_trans. eapply image_apply_r_set_list.  eassumption.  *)
-                   admit. (* change FV subset to include fvs in fm *)
-                ** intros. eapply preord_exp_app_l.
-                   --- admit.
-                   --- admit. 
-                   --- intros. assert (Heqf' := Heqf). eapply H6 in Heqf. destructAll.
-                       do 2 subst_exp. eapply H4.
-                       admit. 
-                       eapply fun_map_inv_set_lists.
-                       eapply  fun_map_inv_def_funs.
-                       eassumption.
-                       admit.
-                       (* eapply Disjoint_sym. eapply Disjoint_Included_r; [| eassumption ]. *)
-                       
-                       normalize_bound_var. 
-                       H4. 
-                normalize_occurs_free; sets.
-             split.
-             
-      simpl. 
-       eapply bind_triple.
-          pre
-          reflexivity. 
-        rewrite Union_Setminus with (S1 := occurs_free e) (S2 := [set v]).
-        2:{ 
+        *  eapply return_triple.
+           intros. split; [| split; [| split; [| split ]]]; try eassumption.
+           ++ constructor.
+           ++ simpl. repeat normalize_occurs_free. rewrite !image_Union, image_Singleton.
+              rewrite FromList_apply_list. sets.
+           ++ normalize_bound_var. sets.
+           ++ intros. eapply preord_exp_app_compat.
+              assumption. assumption.
+              eapply H0. now constructor.
+              eapply Forall2_preord_var_env_map. eassumption.
+              now constructor.
+    - (* Eprim *)
+      admit.
+      
