theories/L6_PCPS/shrink_cps_correct.v
@@ -113,7 +113,7 @@ Inductive gen_rw : relation exp :=
 
 Definition gr_clos n := refl_trans_closure_n gen_rw n.
 
-Section Shrink_correct.
+Section Shrink_correct. 
 
   Variable pr : prims.
   Variable cenv : ctor_env.
@@ -1352,20 +1352,6 @@ Section Shrink_correct.
   Qed.
 
 
-  Lemma preord_env_P_inj_set_l_apply_r S k rho1 rho2 m x y v v' : 
-    preord_env_P_inj cenv PG (S \\ [set x]) k (apply_r m) rho1 rho2 ->
-    M.get y rho2 = Some v' ->
-    preord_val cenv PG k v v' ->
-    preord_env_P_inj cenv PG S k (apply_r (M.set x y m)) (map_util.M.set x v rho1) rho2.
-  Proof.
-    intros Henv Hg1 Hval z Hin v1 Hgetz.
-    destruct (peq z x); subst.
-    - eexists. unfold apply_r. rewrite M.gss in *. inv Hgetz. split; eauto.
-    - unfold apply_r. rewrite M.gso in *; eauto.
-      eapply Henv; eauto. constructor; eauto.
-      intros Hc; inv Hc; eauto.
-  Qed.
-
   Lemma preord_env_P_inj_id S k rho1 rho2 : 
     preord_env_P cenv PG S k rho1 rho2 ->
     preord_env_P_inj cenv PG S k id rho1 rho2.
@@ -1493,39 +1479,6 @@ Section Shrink_correct.
         inv H0. intro.
         apply H3. left. auto.
     -   intros. inv H.
-  Qed.
-  
-  Lemma preord_env_P_inj_set_lists_l S k rho1 rho1' rho2 xs ys vs1 vs2 : 
-    preord_env_P cenv PG (S \\ FromList xs) k rho1 rho2 ->
-
-    set_lists xs vs1 rho1 = Some rho1'  ->
-    get_list ys rho2 = Some vs2 ->
-    Forall2 (preord_val cenv PG k) vs1 vs2 ->      
-
-    preord_env_P_inj cenv PG S k (apply_r (set_list (combine xs ys) (M.empty var))) rho1' rho2.
-  Proof.
-    revert S k rho1 rho1' rho2 ys vs1 vs2; induction xs;
-      intros S k rho1 rho1' rho2 ys vs1 vs2 Henv Hset Hget Hvall.
-    - simpl in Hset. destruct vs1; try congruence. inv Hset.
-      inv Hvall. destruct ys; simpl in Hget; try congruence.
-      intros z Hin v1 Hgetz. unfold apply_r. rewrite M.gempty. eapply Henv.
-      constructor; eauto. eassumption.
-
-      destruct (M.get e rho2); try congruence.
-      destruct (get_list ys rho2); try congruence.
-    - simpl in Hset. destruct vs1; try congruence.
-      destruct vs2 as [|v' vs2]; inv Hvall.
-      destruct (set_lists xs vs1 rho1) eqn:Hset1'; try congruence. inv Hset.
-      destruct ys as [| y ys]; simpl in Hget; try congruence. 
-      destruct (M.get y rho2) eqn:Hgety; try congruence.
-      destruct (get_list ys rho2) eqn:Hgetys; try congruence.
-      inv Hget. simpl. 
-
-      eapply preord_env_P_inj_set_l_apply_r; [| eassumption | eassumption ]. 
-
-      eapply IHxs. eapply preord_env_P_antimon. eassumption.
-      normalize_sets. rewrite Setminus_Union. sets.
-      eassumption. eassumption. eassumption. 
   Qed.
 
   Lemma image'_get_set_list S xs1 vs1 :
